src/AADL/legality/all.v
@@ -34,8 +34,7 @@ Require Export Oqarina.AADL.legality.component_wf.
 Require Export Oqarina.AADL.legality.connections_wf.
 Require Export Oqarina.AADL.legality.features_wf.
 Require Export Oqarina.AADL.legality.properties_wf.
-
-Create HintDb aadl_wf.
+Require Import Oqarina.core.tactics.
 
 Global Hint Resolve
     Well_Formed_Component_Type_Interface_dec
@@ -45,5 +44,4 @@ Global Hint Resolve
     Well_Formed_Component_Features_dec
     Well_Formed_Property_Associations_dec
     Rule_4_5_N1_dec
-: aadl_wf.
-
+: well_know_wf_dec.
